proofs in RedAll.

theories/Lambda/RedAll.v
@@ -13,7 +13,7 @@ Require Import FunctionalExtensionality.
 Set Implicit Arguments.
 Set Strict Implicit.
 
-Section beta_all.
+Section reducer.
   Context {sym : Type}.
   Context {typ : Type}.
   Context {RT : RType typ}
@@ -26,12 +26,200 @@ Section beta_all.
 
   Context {ED_typ : EqDec _ (@eq typ)}.
 
-  (** NOTE: I should extend [delta] with [vars]
-   ** - that means that its specification is exactly the same as [beta_all]
-   **)
-  Variable delta : expr typ sym -> list (expr typ sym) -> expr typ sym.
+  Fixpoint var_termsD tus tvs n (ls : list (option (expr typ sym)))
+  : option (ExprI.exprT tus tvs Prop) :=
+    match ls with
+      | nil => Some (fun _ _ => True)
+      | None :: ls => var_termsD tus tvs (S n) ls
+      | Some l :: ls =>
+        match var_termsD tus tvs (S n) ls
+            , nth_error_get_hlist_nth typD tvs n
+        with
+          | Some vsD , Some (existT t get) =>
+            match exprD' tus tvs t l with
+              | None => None
+              | Some vD => Some (fun us vs => get vs = vD us vs /\ vsD us vs)
+            end
+          | None , _ => None
+          | _ , None => None
+        end
+    end.
 
-  Fixpoint get_var (v : nat) (ls : list (option (expr typ sym))) (acc : nat)
+  Theorem var_termsD_sem tus tvs
+  : forall ls n P,
+      var_termsD tus tvs n ls = Some P ->
+      (forall u e,
+         nth_error ls u = Some (Some e) ->
+         exists t get (vD : ExprI.exprT tus tvs (typD t)),
+           nth_error_get_hlist_nth typD tvs (n + u) = Some (@existT _ _ t get) /\
+           exprD' tus tvs t e = Some vD /\
+           forall us vs,
+             P us vs -> get vs = vD us vs).
+  Proof.
+    induction ls; simpl; intros; inv_all.
+    - subst. exfalso.
+      destruct u; simpl in *; inversion H0.
+    - destruct u.
+      + simpl in *. inversion H0; clear H0; subst.
+        forward. inv_all; subst.
+        cutrewrite (n + 0 = n); [ | omega ].
+        do 3 eexists; split; eauto; split; eauto.
+        intros. tauto.
+      + simpl in H0.
+        cutrewrite (n + S u = (S n) + u); [ | omega ].
+        destruct a; eauto.
+        forward; inv_all; subst.
+        specialize (IHls _ _ H _ _ H0).
+        forward_reason.
+        do 3 eexists; split; eauto. split; eauto.
+        firstorder.
+  Qed.
+
+  (** I want this to capture the fact that when the entry is [Some], then
+   ** the "resulting environment" does not contain the entry.
+   ** 1) State a relation between the pre- and post-environments
+   **    (i.e. the hlists)
+   **)
+  Inductive var_termsP
+  : forall (tus tvs tus' tvs' : tenv typ),
+      list (option (expr typ sym)) ->
+      ExprI.exprT tus tvs (ExprI.exprT tus' tvs' Prop) ->
+      Prop :=
+  | var_termsP_nil
+    : forall tus tvs (P : ExprI.exprT tus tvs (ExprI.exprT tus tvs Prop)),
+        (forall us vs us' vs', P us vs us' vs' -> us = us' /\ vs = vs') ->
+        @var_termsP tus tvs tus tvs nil P
+  | var_termsP_cons_None
+    : forall t tus tvs tus' tvs' p
+             (P : ExprI.exprT tus (t :: tvs) (ExprI.exprT tus' (t :: tvs') Prop))
+             (P' : ExprI.exprT tus tvs (ExprI.exprT tus' tvs' Prop)),
+        @var_termsP tus tvs tus' tvs' p P' ->
+        (forall us (vs : HList.hlist typD (t :: tvs))
+                us' (vs' : HList.hlist typD (t :: tvs')),
+           P us vs us' vs' ->
+           hlist_hd vs = hlist_hd vs' /\
+           P' us (hlist_tl vs) us' (hlist_tl vs')) ->
+        @var_termsP tus (t :: tvs) tus' (t :: tvs') (None :: p) P
+  | var_termsP_cons_Some
+    : forall t tus tvs tus' tvs' p e eD
+             (P : ExprI.exprT tus (t :: tvs) (ExprI.exprT tus' tvs' Prop))
+             (P' : ExprI.exprT tus tvs (ExprI.exprT tus' tvs' Prop)),
+        @var_termsP tus tvs tus' tvs' p P' ->
+        exprD' tus' tvs' t e = Some eD ->
+        (forall us (vs : HList.hlist typD (t :: tvs))
+                us' (vs' : HList.hlist typD tvs'),
+           P us vs us' vs' ->
+           P' us (hlist_tl vs) us' vs' /\
+           hlist_hd vs = eD us' vs') ->
+        @var_termsP tus (t :: tvs) tus' tvs' (Some e :: p) P.
+
+  Instance Injective_var_termsP t var_terms tus tvs tus' tvs' P
+  : Injective (@var_termsP tus (t :: tvs) tus' (t :: tvs')
+                           (@None (expr typ sym) :: var_terms)
+                           P) :=
+    {| result := exists P',
+                   @var_termsP tus tvs tus' tvs' var_terms P' /\
+                   (forall us (vs : HList.hlist typD (t :: tvs))
+                           us' (vs' : HList.hlist typD (t :: tvs')),
+                      P us vs us' vs' ->
+                      hlist_hd vs = hlist_hd vs' /\
+                      P' us (hlist_tl vs) us' (hlist_tl vs')) |}.
+  Proof.
+    refine (fun H =>
+              match H in @var_termsP a b c d X P
+                    return match b as b , d as d , X
+                                 return ExprI.exprT a b (ExprI.exprT c d Prop) -> Prop
+                           with
+                             | t :: b , t' :: d , None :: var_terms =>
+                               fun P => forall pf : t = t' ,
+                                        exists P',
+                                          @var_termsP a b c d var_terms P' /\
+                                          (forall (us : HList.hlist typD a) (vs : HList.hlist typD (t :: b))
+                                                  (us' : HList.hlist typD c) (vs' : HList.hlist typD (t' :: d)),
+                                             P us vs us' vs' ->
+                                             hlist_hd vs = match eq_sym pf in _ = t return typD t with
+                                                             | eq_refl => hlist_hd vs'
+                                                           end /\
+                                             P' us (hlist_tl vs) us' (hlist_tl vs')) 
+                             | _ , _ , _ => fun _ => True
+                           end P
+              with
+                | var_termsP_cons_None _ _ _ _ _ _ _ _ _ _ => _
+                | _ => _
+              end eq_refl); try solve [ destruct tvs'0 ; tauto | destruct tvs0 ; tauto ].
+    intros.
+    exists P'. split; auto.
+    intros.
+    eapply a in H0. destruct H0; clear a.
+    split; auto.
+    rewrite (UIP_refl pf). apply H0.
+  Defined.
+
+
+  Definition full_reducer : Type :=
+    forall (vars : list (option (expr typ sym)))
+           (e : expr typ sym)
+           (args : list (expr typ sym)), expr typ sym.
+  Require Import MirrorCore.SubstI.
+
+  Fixpoint applys {ts : tenv typ} {t : typ}
+           (xs : hlist typD ts) : typD (fold_right (@typ2 _ _ Fun _) t ts) -> typD t :=
+    match xs in hlist _ ts return typD (fold_right (@typ2 _ _ Fun _) t ts) -> typD t with
+      | Hnil => fun f => f
+      | Hcons t' ts' x xs => fun f =>
+        @applys ts' t xs (match typ2_cast t' (fold_right (@typ2 _ _ Fun _) t ts') in _ = t return t with
+                            | eq_refl => f
+                          end x)
+    end.
+
+  Definition full_reducer_ok (red : full_reducer) : Prop :=
+    forall e var_terms tus tvs tus' tvs' P,
+      @var_termsP tus tvs tus' tvs' var_terms P ->
+      (** TODO: This is wrong, the [es] have already been converted to
+       ** [tus',tvs']
+       **)
+      forall es t targs fD esD,
+      let arrow_type := fold_right (@typ2 _ _ Fun _) t targs in
+      exprD' tus tvs arrow_type e = Some fD ->
+      hlist_build (fun t => ExprI.exprT tus' tvs' (typD t))
+                  (fun t e => exprD' tus' tvs' t e) targs es = Some esD ->
+      exists val',
+        exprD' tus' tvs' t (red var_terms e es) = Some val' /\
+        forall us vs us' vs',
+          P us vs us' vs' ->
+          applys
+            (hlist_map (fun t (x : ExprI.exprT tus' tvs' (typD t)) => x us' vs') esD)
+            (fD us vs) = val' us' vs'.
+
+  Definition partial_reducer : Type :=
+    forall (e : expr typ sym)
+           (args : list (expr typ sym)), expr typ sym.
+  (** TODO: This pattern seems common enough to warrent something
+   ** interesting
+   **)
+  Definition partial_reducer_ok (red : partial_reducer) : Prop :=
+    forall e es t tus tvs val P,
+      exprD' tus tvs t (apps e es) = Some val ->
+      exists val',
+        exprD' tus tvs t (red e es) = Some val' /\
+        forall us vs,
+          P us vs ->
+          val us vs = val' us vs.
+
+  Definition apps_reducer : partial_reducer :=
+    @apps typ sym.
+
+  Theorem apps_partial_reducer_ok : partial_reducer_ok apps_reducer.
+  Proof.
+    unfold apps_reducer; red. intros. eauto.
+  Qed.
+
+  (** [acc] is the amount to lift by
+   ** this is because there is some fancyness going on since applied lambdas
+   ** actually remove entries from the environment
+   **)
+  Fixpoint get_var (v : nat) (ls : list (option (expr typ sym)))
+           (acc : nat) {struct ls}
   : expr typ sym :=
     match ls with
       | nil => Var (acc + v)
@@ -47,359 +235,314 @@ Section beta_all.
         end
     end.
 
-(*
+  Let exprD'_conv :=
+    @ExprI.exprD'_conv typ RT (expr typ sym) (@Expr_expr typ sym RT _ _).
+
   Lemma get_var_ok
-  : forall n ls v e,
-      get_var n ls v =
-      (e = Var (n + v)) \/
-      True.
+  : forall tus tvs tus'  tvs' var_terms P,
+      @var_termsP tus tvs tus' tvs' var_terms P ->
+      forall _tvs _tvs' v t val,
+      let acc := length _tvs' in
+        exprD' tus (_tvs ++ tvs) t (Var (length _tvs + v)) = Some val ->
+        exists val',
+          exprD' tus' (_tvs' ++ tvs') t (get_var v var_terms acc) = Some val' /\
+          forall us _vs vs us' _vs' vs',
+            P us vs us' vs' ->
+            val us (hlist_app _vs vs) =
+            val' us' (hlist_app _vs' vs').
   Proof.
-    induction n; simpl.
-    - destruct ls; simpl; intros.
-      + left. rewrite Plus.plus_0_r in H. auto.
-      + destruct o.
-        * admit.
-        * left. auto.
-    - destruct ls; simpl; do 2 intro.
-      + rewrite <- plus_n_Sm. rewrite Plus.plus_comm.
-        left; auto.
-      + destruct o.
-        * specialize (IHn ls (S v) _ eq_refl).
-
-             *
-*)
-
-  Fixpoint beta_all
-           (args : list (expr typ sym))
-           (vars : list (option (expr typ sym)))
-           (e : expr typ sym) : expr typ sym :=
-    match e with
-      | App e' e'' =>
-        beta_all (beta_all nil vars e'' :: args) vars e'
-      | Abs t e' =>
-        match args with
-          | nil => Abs t (beta_all nil (None :: vars) e') (** args = nil **)
-          | a :: args => beta_all args (Some a :: vars) e'
-        end
-      | Var v =>
-        delta (get_var v vars 0) args
-      | e => delta e args
-    end.
-
-  (** the default delta function is [apps] **)
-  Definition delta_sound
-  := forall e es tus tvs t val,
-       exprD' tus tvs t (apps e es) = Some val ->
-       exists val',
-         exprD' tus tvs t (delta e es) = Some val' /\
-         forall us vs,
-           val us vs = val' us vs.
-
-  Hypothesis deltaOk : delta_sound.
-
-  Inductive EnvForall {A} (R : A -> forall t : typ, typD t -> Prop)
-  : list A -> forall tvs, hlist typD tvs -> Prop :=
-  | EnvForall_nil : EnvForall R nil Hnil
-  | EnvForall_cons : forall e es t ts v vs,
-                       R e t v ->
-                       @EnvForall A R es ts vs ->
-                       @EnvForall A R (e :: es) (t :: ts) (Hcons v vs).
-
-  Lemma Forall2_sem2
-  : forall T U (P : T -> U -> Prop) xs ys,
-      Forall2 P xs ys ->
-      forall v y,
-        nth_error ys v = Some y ->
-        exists x, nth_error xs v = Some x /\
-                  P x y.
-  Proof.
-    clear. induction 1; simpl; intros.
-    { destruct v; inversion H. }
-    { destruct v.
-      { simpl in *. eexists; split; eauto.
-        inversion H1. subst. auto. }
-      { simpl in *. eauto. } }
-  Qed.
-
-  Section Forall2i.
-    Variables T U : Type.
-
-    Section def.
-      Variable P : nat -> T -> U -> Prop.
-
-      Inductive Forall2i : nat -> list T -> list U -> Prop :=
-      | F2i_nil : forall n, Forall2i n nil nil
-      | F2i_cons : forall x xs y ys n, P n x y ->
-                                       Forall2i (S n) xs ys ->
-                                       Forall2i n (x :: xs) (y :: ys).
-    End def.
-
-    Variable P Q : nat -> T -> U -> Prop.
-    Lemma Forall2i_shift
-    : forall m n xs ys,
-        (forall n x y, P n x y -> Q (m + n) x y) ->
-        Forall2i P n xs ys ->
-        Forall2i Q (m + n) xs ys.
-    Proof.
-      clear. induction 2.
-      { constructor. }
-      { constructor; eauto.
-        replace (m + S n) with (S (m + n)) in IHForall2i by omega.
-        assumption. }
-    Qed.
-  End Forall2i.
-
-(*
-  Lemma beta_all_respectful
-  : forall args args' vars vars' e e',
-      Forall
-      beta_all args vars e =
-      beta_all args' vars' e'
-*)
-
-  Lemma exprD'_App_Abs
-  : forall tus tvs t t0 e ex val,
-      exprD' tus tvs t0 (App (Abs t e) ex) = Some val ->
-      exprD' tus tvs t0 (substitute_one 0 ex e) = Some val.
-  Proof.
-    intros.
-    autorewrite with exprD_rw in *; simpl in *.
-    forward.
-    autorewrite with exprD_rw in *; simpl in *.
-    inv_all; subst.
-    rewrite typ2_match_zeta in H0; eauto.
-    rewrite eq_option_eq in H0.
-    forward. inv_all; subst.
-    destruct r.
-    generalize (@substitute_one_sound _ _ _ _ _ _ _ _ _ tus e nil ex _ eq_refl tvs t1 t0).
-    simpl. Cases.rewrite_all_goal.
-    intros. forward.
-    f_equal. unfold exprT_App.
-    autorewrite with eq_rw.
-    clear - H4.
-    apply functional_extensionality; intro.
-    apply functional_extensionality; intro.
-    repeat first [ rewrite eq_Const_eq | rewrite eq_Arr_eq ].
-    specialize (H4 x Hnil x0).
-    simpl in *.
-    autorewrite with eq_rw. auto.
-  Qed.
-
-  Lemma Forall2i_nth_snd
-  : forall T U (P : nat -> T -> U -> Prop) i xs ys,
-      Forall2i P i xs ys ->
-      forall n y,
-        nth_error ys n = Some y ->
-        exists x, nth_error xs n = Some x /\
-                  P (i + n) x y.
-  Proof.
-    induction 1.
-    - intros ? ?; rewrite nth_error_nil. congruence.
-    - destruct n0; simpl; intros.
-      + eexists; split; eauto.
-        rewrite Plus.plus_0_r. inv_all.
-        subst. assumption.
-      + rewrite <- plus_n_Sm.
-        simpl in *. auto.
-  Qed.
-
-  Lemma apply_sem_same
-  : forall tus tvs args t f f' t' val val',
-      apply_sem' (tus := tus) (tvs := tvs) T2 RS t f args t' = Some val ->
-      apply_sem' T2 RS t f' args t' = Some val' ->
-      forall us vs,
-        f us vs = f' us vs ->
-        val us vs = val' us vs.
-  Proof.
-    induction args.
-    + simpl.
-      intros. forward. inv_all. subst.
-      unfold Rcast, Relim.
-      autorewrite with eq_rw.
-      rewrite H1. reflexivity.
-    + simpl. intros.
-      arrow_case t.
-    - unfold Relim in *; autorewrite with eq_rw in *.
-      forward.
-      specialize (IHargs _ _ _ _ _ _ H0 H3); clear H0 H3.
-      simpl in *. eapply IHargs.
-      autorewrite with eq_rw.
-      rewrite H1. reflexivity.
-    - congruence.
-  Qed.
-
-  Lemma apply_sem'_same_args_safe
-  : forall tus tvs args t f f' t' val,
-      apply_sem' (tus := tus) (tvs := tvs) T2 RS t f args t' = Some val ->
-      exists val', apply_sem' (tus := tus) (tvs := tvs) T2 RS t f' args t' = Some val'.
-  Proof.
-    induction args; simpl; intros.
-    + forward. eauto.
-    + arrow_case t.
-      unfold Relim in *.
-      autorewrite with eq_rw in *.
-      forward.
-      eapply IHargs in H1. eapply H1. congruence.
-  Qed.
-
-  Inductive EnvModels tus (us : hlist typD tus)
-  : forall tvs, list (option (expr typ sym)) -> hlist typD tvs -> Prop :=
-  | EnvModels_nil : @EnvModels tus us nil nil Hnil
-  | EnvModels_None : forall t tvs vs val vals,
-                       @EnvModels tus us tvs vs vals ->
-                       @EnvModels tus us (t :: tvs) (None :: vs) (Hcons val vals)
-  | EnvModels_Some : forall t tvs e vs val vals val',
-                       exprD' tus tvs t e = Some val' ->
-                       val' us vals = val ->
-                       @EnvModels tus us tvs vs vals ->
-                       @EnvModels tus us (t :: tvs) (Some e :: vs) (Hcons val vals).
-
-(*
-  Theorem beta_all_sound
-  : forall tus e tvs t val args vars,
-      Forall2i (fun n t e =>
-                  match e with
-                    | None => True
-                    | Some e =>
-                      exists val, exprD' ts tus (skipn (S n) tvs) t e = Some val
-                  end) 0 tvs vars ->
-      exprD' ts tus tvs t (apps (substitute e) args) = Some val ->
-      exists val',
-        exprD' ts tus tvs t (beta_all args vars e) = Some val' /\
-        forall us vs,
-          @EnvModels tus us tvs vars vs ->
-          val us vs = val' us vs.
-
-
-  (** TODO: This is not true **)
-  Theorem beta_all_sound
-  : forall tus e tvs t val args vars,
-      Forall2i (fun n t e => match e with
-                               | None => True
-                               | Some e =>
-                                 exists val, exprD' ts tus (skipn (S n) tvs) t e = Some val
-                             end) 0 tvs vars ->
-      exprD' ts tus tvs t (apps e args) = Some val ->
-      exists val',
-        exprD' ts tus tvs t (beta_all args vars e) = Some val' /\
-        forall us vs,
-          @EnvModels tus us tvs vars vs ->
-          val us vs = val' us vs.
-  Proof.
-    induction e; simpl; intros.
-    { rewrite exprD'_apps in H0; eauto.
-      unfold apps_sem' in H0. forward.
-      autorewrite with exprD_rw in H1. simpl in H1.
-      forward. inv_all; subst.
-      simpl in H0. destruct r.
-      clear H4. unfold Rcast_val, Rcast, Relim, Rsym in H2. simpl in H2.
-      { admit. } }
-    { eapply deltaOk in H0.
-      destruct H0 as [ ? [ ? ? ] ].
-      eexists; split; eauto. }
-    { generalize H0.
-      rewrite exprD'_apps in H0; eauto.
-      unfold apps_sem' in H0.
-      forward.
-      autorewrite with exprD_rw in *; simpl in *; forward.
-      change e2 with (apps e2 nil) in H5.
-      eapply IHe2 with (vars := vars) in H5; eauto; clear IHe2.
+    induction 1; simpl; intros.
+    { revert H0.
+      autorewrite with exprD_rw. simpl.
+      intros; forward; inv_all; subst.
+      eapply nth_error_get_hlist_nth_appR in H1; [ | omega ]. simpl in H1.
+      replace (length _tvs + v - length _tvs) with v in H1 by omega.
       forward_reason.
-      assert (exists val',
-                exprD' ts tus tvs t (apps (App e1 (beta_all nil vars e2)) args) = Some val' /\
-             forall us vs,
-               @EnvModels tus us tvs vars vs ->
-               val us vs = val' us vs).
-      { rewrite exprD'_apps; eauto.
-        unfold apps_sem'. simpl.
+      assert (length _tvs' + v >= length _tvs') by omega.
+      generalize (@nth_error_get_hlist_nth_rwR typ typD _tvs' tvs _ H3).
+      replace (length _tvs' + v - length _tvs') with v by omega.
+      rewrite H0.
+      intros; forward_reason; Cases.rewrite_all_goal.
+      eexists; split; eauto.
+      simpl. intros. f_equal. etransitivity. eapply H1.
+      apply H in H6. destruct H6; subst. eauto. }
+    { destruct v.
+      { rewrite Plus.plus_0_r in *.
+        revert H1. autorewrite with exprD_rw. simpl.
+        clear IHvar_termsP.
+        intros; forward; inv_all; subst.
+        assert (length _tvs' >= length _tvs') by omega.
+        generalize (@nth_error_get_hlist_nth_rwR typ typD _tvs' (t :: tvs') _ H1).
+        rewrite Minus.minus_diag. simpl.
+        intros; forward_reason.
         Cases.rewrite_all_goal.
-        assert (typeof_expr ts tus tvs (beta_all nil vars e2) = Some t1) by admit.
-        Cases.rewrite_all_goal.
-        autorewrite with exprD_rw. simpl.
-        Cases.rewrite_all_goal.
-        inv_all; subst.
-        consider (apply_sem' T2 RS t0 (Open_App o0 x) args t); intros.
-        { eexists; split; eauto.
+        eapply nth_error_get_hlist_nth_appR in H2; [ | omega ]. simpl in *.
+        rewrite Minus.minus_diag in H2. simpl.
+        forward_reason; inv_all; subst.
+        rewrite H3.
+        eexists; split; eauto.
+        simpl; intros. f_equal.
+        rewrite H6; clear H6.
+        subst. apply H0 in H2; clear H0.
+        destruct H2. etransitivity; eauto. }
+      { revert H1.
+        specialize (IHvar_termsP (_tvs ++ t :: nil) (_tvs' ++ t :: nil) v t0).
+        revert IHvar_termsP.
+        autorewrite with exprD_rw.
+        simpl. intros.
+        forward. inv_all; subst.
+        eapply nth_error_get_hlist_nth_appR in H2; [ | omega ].
+        simpl in *.
+        replace (length _tvs + S v - length _tvs) with (S v) in H2; [ | omega ].
+        forward_reason.
+        forward; inv_all; subst.
+        assert (length (_tvs ++ t :: nil) + v >= length (_tvs ++ t :: nil)) by omega.
+        subst.
+        generalize (@nth_error_get_hlist_nth_rwR _ typD (_tvs ++ t :: nil) tvs (length (_tvs ++ t :: nil) + v) H1).
+        replace (length (_tvs ++ t :: nil) + v - length (_tvs ++ t :: nil)) with v by omega.
+        rewrite H4. intros; forward_reason.
+        revert IHvar_termsP.
+        rewrite H5. rewrite H3. intro IH.
+        specialize (IH _ eq_refl).
+        forward_reason.
+        rewrite app_length in H7. simpl in H7.
+        rewrite Plus.plus_comm in H7. simpl in H7.
+        rewrite exprD'_conv
+           with (pfu := eq_refl) (pfv := eq_sym (app_ass_trans _ _ _)) in H7.
+        autorewrite with eq_rw in H7.
+        forward; inv_all; subst.
+        simpl in *. eexists; split; eauto.
+        intros.
+        eapply H0 in H9; clear H0.
+        destruct H9.
+        rewrite H2; clear H2.
+        specialize (H8 us (hlist_app _vs (fst (hlist_split (t :: nil) tvs vs)))
+                       (snd (hlist_split (t :: nil) tvs vs)) us'
+                       (hlist_app _vs' (fst (hlist_split (t :: nil) tvs' vs')))
+                       (snd (hlist_split (t :: nil) tvs' vs'))).
+        eapply H8 in H9; clear H8; simpl in *.
+        rewrite <- H6 in H9; clear H6.
+        rewrite H9; clear H9.
+        autorewrite with eq_rw.
+        f_equal. rewrite hlist_app_assoc.
+        clear.
+        rewrite Eq.match_eq_sym_eq'.
+        f_equal.
+        symmetry. apply (hlist_eta vs'). } }
+    { destruct v.
+      { clear IHvar_termsP.
+        generalize (@exprD'_lift typ sym _ _ _ _ _ _ tus' e nil _tvs' tvs' t).
+        simpl. rewrite H0. intros; forward.
+        assert (t = t0).
+        { revert H2.
+          autorewrite with exprD_rw. clear.
+          simpl; intros; forward.
+          clear H2. subst.
+          eapply nth_error_get_hlist_nth_appR in H0; [ | omega ].
+          simpl in H0.
+          replace (length _tvs + 0 - length _tvs) with 0 in H0 by omega.
+          forward_reason.
+          inv_all. subst. apply r. }
+        subst.
+        eexists; split; eauto.
+        intros. specialize (H4 us' Hnil _vs' vs').
+        simpl in H4.
+        autorewrite with exprD_rw in H2.
+        simpl in H2.
+        forward; inv_all; subst.
+        eapply H1 in H5; clear H1.
+        rewrite <- H4; clear H4.
+        destruct H5. rewrite <- H2; clear H2.
+        eapply nth_error_get_hlist_nth_appR in H6; [ | omega ].
+        simpl in *.
+        replace (length _tvs + 0 - length _tvs) with 0 in H6 by omega.
+        forward_reason; inv_all; subst.
+        rewrite H4; clear H4.
+        subst.
+        red in r.
+        rewrite (UIP_refl r). reflexivity. }
+      { revert H2.
+        specialize (IHvar_termsP (_tvs ++ t :: nil) _tvs' v t0).
+        revert IHvar_termsP.
+        autorewrite with exprD_rw.
+        simpl. intros.
+        forward. inv_all; subst.
+        eapply nth_error_get_hlist_nth_appR in H3; [ | omega ].
+        simpl in *.
+        replace (length _tvs + S v - length _tvs) with (S v) in H3; [ | omega ].
+        forward_reason.
+        forward; inv_all; subst.
+        assert (length (_tvs ++ t :: nil) + v >= length (_tvs ++ t :: nil)) by omega.
+        subst.
+        generalize (@nth_error_get_hlist_nth_rwR _ typD (_tvs ++ t :: nil) tvs (length (_tvs ++ t :: nil) + v) H2).
+        replace (length (_tvs ++ t :: nil) + v - length (_tvs ++ t :: nil)) with v by omega.
+        rewrite H5. intros; forward_reason.
+        revert IHvar_termsP.
+        rewrite H6. rewrite H4. intro IH.
+        specialize (IH _ eq_refl).
+        forward_reason.
+        forward; inv_all; subst.
+        simpl in *. eexists; split; eauto.
+        intros.
+        eapply H1 in H10; clear H1.
+        destruct H10.
+        specialize (H9 us (hlist_app _vs (fst (hlist_split (t :: nil) tvs vs)))
+                       (snd (hlist_split (t :: nil) tvs vs)) us' _vs' vs').
+        simpl in H9. eapply H9 in H1; clear H9.
+        rewrite H3; clear H3.
+        erewrite H7; clear H7.
+        eapply H1. } }
+  Qed.
+
+  Section beta_all.
+    Variable rec : full_reducer.
+
+    Fixpoint beta_all_gen
+             (vars : list (option (expr typ sym)))
+             (e : expr typ sym)
+             (args : list (expr typ sym)) : expr typ sym :=
+      match e with
+        | App e' e'' =>
+          beta_all_gen vars e' (beta_all_gen vars e'' nil :: args)
+        | Abs t e' =>
+          match args with
+            | nil => Abs t (beta_all_gen (None :: vars) e' nil) (** args = nil **)
+            | a :: args => beta_all_gen (Some a :: vars) e' args
+          end
+        | Var v =>
+          (** [get_var] has already done the conversion! **)
+          rec nil (get_var v vars 0) args
+        | e => rec vars e args
+      end.
+
+    Hypothesis rec_sound : full_reducer_ok rec.
+
+    Theorem beta_all_gen_sound : full_reducer_ok beta_all_gen.
+    Proof.
+      red. induction e; try solve [ simpl; intros; eauto ].
+      { (* Var *)
+        simpl; intros.
+        generalize (@get_var_ok _ _ _ _ _ _ H nil nil v _ _ H0).
+        clear H0; intros.
+        forward_reason. simpl in *.
+        eapply rec_sound in H0; eauto.
+        Focus 2. eapply var_termsP_nil.
+        intros. eapply H3.
+        eapply H0 in H1; clear H0.
+        forward_reason.
+        eexists; split; eauto. intros.
+        eapply H2 with (_vs := Hnil) (_vs' := Hnil) in H3.
+        specialize (H1 us' vs' us' vs' (conj eq_refl eq_refl)).
+        simpl in *. rewrite H3. eapply H1. }
+      { (* App *)
+        simpl; intros.
+        autorewrite with exprD_rw in H0. simpl in H0.
+        forward; inv_all; subst.
+        specialize (IHe2 var_terms tus tvs tus' tvs' _ H nil t0 nil _ _ H3 eq_refl).
+        forward_reason.
+        specialize (@IHe1 var_terms _ _ _ _ _ H (beta_all_gen var_terms e2 nil :: es) _ (t0 :: targs) _
+                          (@Hcons _ _ t0 _ x esD) H2).
+        simpl in IHe1.
+        rewrite H1 in IHe1.
+        rewrite H4 in IHe1. specialize (IHe1 eq_refl).
+        forward_reason.
+        eexists; split; eauto.
+        intros.
+        specialize (H5 _ _ _ _ H8).
+        specialize (H7 _ _ _ _ H8).
+        rewrite <- H5 in H7; clear H5. simpl in H7.
+        unfold exprT_App.
+        match goal with
+          | H : context [ match ?X with _ => _ end ]
+            |- context [ match eq_sym ?Y with _ => _ end ] =>
+            change Y with X; generalize dependent X
+        end.
+        clear.
+        generalize dependent (typD (typ2 t0 (fold_right (typ2 (F:=Fun)) t targs))).
+        intros; subst. simpl in *. eauto. }
+      { (* Abs *)
+        simpl; intros.
+        destruct es.
+        { destruct targs; simpl in *; try congruence.
+          inv_all; subst.
+          revert H0.
+          autorewrite with exprD_rw; simpl.
           intros.
-          specialize (H8 _ _ H10).
-          clear H2 H10 H.
-          apply (apply_sem_same _ _ _ _ _ H3 H6 us vs).
-          unfold Open_App.
-          unfold Relim, OpenT, ResType.OpenT.
-          repeat first [ rewrite eq_Const_eq | rewrite eq_Arr_eq ].
-          rewrite H8. reflexivity. }
-        { exfalso.
-          eapply apply_sem'_same_args_safe in H3.
-          destruct H3. rewrite H3 in H6. congruence. } }
-      { destruct H9 as [ ? [ ? ? ] ].
-        change (apps (App e1 (beta_all nil vars e2)) args)
-          with (apps e1 (beta_all nil vars e2 :: args)) in H9.
-        eapply IHe1 in H9; eauto.
-        forward_reason. eexists; split; eauto.
-        intros. rewrite <- H11; eauto. } }
-    { destruct args.
-      { simpl in *.
-        autorewrite with exprD_rw in *; simpl in *.
-        arrow_case ts t0.
-        { clear H1. red in x1. subst. simpl in *.
-          rewrite eq_option_eq in *.
-          forward. inv_all; subst.
-          change e with (apps e nil) in H2.
-          eapply IHe with (vars := None :: vars) in H2; eauto.
-          { forward_reason. Cases.rewrite_all_goal.
-            eexists; split; eauto.
-            intros.
-            unfold OpenT, ResType.OpenT.
-            repeat first [ rewrite eq_Const_eq | rewrite eq_Arr_eq ].
-            match goal with
-              | |- match ?X with _ => _ end = match ?Y with _ => _ end =>
-                change Y with X ;
-                eapply match_eq_match_eq with (pf := X) (F := fun x => x)
-            end.
-            eapply functional_extensionality.
-            intros.
-            eapply H2.
-            constructor; auto. }
-          { constructor; auto.
-            revert H.
-            eapply (@Forall2i_shift _ _ _ _ 1 0). intros.
-            simpl; auto. } }
-        { congruence. } }
-      { simpl in *.
-        rewrite exprD'_apps in H0; eauto.
-        unfold apps_sem' in H0; eauto. forward.
-        autorewrite with exprD_rw in H1. simpl in H1.
-        forward.
-        assert (Forall2i
-          (fun (n : nat) (t1 : typ) (e1 : option (expr typ sym)) =>
-           match e1 with
-           | Some e2 =>
-               exists val0 : OpenT ts tus (skipn (S n) (t2 :: tvs)) (typD ts t1),
-                 exprD' ts tus (skipn (S n) (t2 :: tvs)) t1 e2 = Some val0
-           | None => True
-           end) 0 (t2 :: tvs) (Some e0 :: vars)).
-        { constructor. simpl. eauto.
-          revert H.
-          eapply (@Forall2i_shift _ _ _ _ 1 0).
-          destruct y; auto. }
-        specialize (fun val => IHe (t2 :: tvs) t0 val (map (lift 0 1) args) (Some e0 :: vars) H6).
-        assert (exists ZZZ, exprD' ts tus (t2 :: tvs) t0 (apps e (map (lift 0 1) args)) = Some ZZZ).
-        { rewrite exprD'_apps; eauto. admit. }
+          arrow_case_any; try congruence.
+          red in x1. subst. simpl in *.
+          revert H0.
+          autorewrite with eq_rw. intros; forward; inv_all; subst.
+          assert (@var_termsP tus (t :: tvs) tus' (t :: tvs')
+                              (None :: var_terms)
+                              (fun us vs us' vs' =>
+                                 P us (hlist_tl vs) us' (hlist_tl vs') /\
+                                 hlist_hd vs = hlist_hd vs')).
+          { eapply var_termsP_cons_None. eassumption.
+            clear. tauto. }
+          specialize (@IHe _ _ _ _ _ _ H2 nil x0 nil _ _ H3 eq_refl).
+          simpl in IHe.
+          forward_reason.
+          rewrite H4.
+          eexists; split; eauto.
+          intros.
+          autorewrite with eq_rw.
+          inv_all.
+          clear H1.
+          apply Data.Eq.match_eq_match_eq with (F := fun x => x).
+          apply functional_extensionality. intros.
+          eapply H5. simpl.
+          split; auto. }
+        { destruct targs; simpl in *; try congruence.
+          forward; inv_all; subst.
+          autorewrite with exprD_rw in H0.
+          rewrite typ2_match_zeta in H0; eauto.
+          simpl in H0.
+          autorewrite with eq_rw in H0.
+          forward; inv_all; subst.
+          destruct r. rename t1 into t.
+          assert (@var_termsP tus (t :: tvs) tus' tvs'
+                              (Some e0 :: var_terms)
+                              (fun us vs us' vs' =>
+                                 P us (hlist_tl vs) us' vs' /\
+                                 hlist_hd vs = e1 us' vs' )).
+          { econstructor; eauto. }
+          specialize (IHe (Some e0 :: var_terms) _ _ _ _ _ H3 es t0 targs _ _ H4 H1).
+          forward_reason.
+          eexists; split; eauto.
+          intros.
+          simpl.
+          specialize (H6 us (Hcons (e1 us' vs') vs) us' vs' (conj H7 eq_refl)).
+          autorewrite with eq_rw.
+          eauto. } }
+    Qed.
 
-admit.
-(*
+    Definition beta_all e := beta_all_gen nil e nil.
 
-        autorewrite with exprD_rw in H3; simpl in H3.
-        rewrite typ2_match_zeta in H3 by eauto.
-        rewrite eq_option_eq in H3. forward.
-        inv_all; subst.
+    Theorem beta_all_sound
+    : forall e t tus tvs val P,
+      exprD' tus tvs t e = Some val ->
+      exists val',
+        exprD' tus tvs t (beta_all e) = Some val' /\
+        forall us vs,
+          P us vs ->
+          val us vs = val' us vs.
+    Proof.
+      intros.
+      Print full_reducer_ok.
+      assert (var_termsP nil
+                         (fun (us : hlist typD tus) (vs : hlist typD tvs)
+                              (us' : hlist typD tus) (vs' : hlist typD tvs) =>
+                            us = us' /\ vs = vs')).
+      { constructor. tauto. }
+      specialize (@beta_all_gen_sound e nil _ _ _ _ _ H0 nil t nil _ _ H eq_refl).
+      simpl.
+      intros. forward_reason.
+      eauto.
+    Qed.
 
-        admit. *) } }
-    { eapply deltaOk in H0.
-      forward_reason. eauto. }
-  Qed. *)
+  End beta_all.
 
-End beta_all.
+End reducer.
 
 (*
 Section test.
